2/new_folder2/__SolToBoogieTest_out.bpl
@@ -65,14 +65,14 @@ call  {:cexpr "msg.sender"} boogie_si_record_sol2Bpl_ref(msgsender_MSG);
 call  {:cexpr "msg.value"} boogie_si_record_sol2Bpl_int(msgvalue_MSG);
 call  {:cexpr "offerPrice"} boogie_si_record_sol2Bpl_int(offerPrice_s58);
 call  {:cexpr "_verisolLastArg"} boogie_si_record_sol2Bpl_bool(true);
-assert {:first} {:sourceFile "/Users/etorres/Proyectos/verisol-test/2/new_folder1/CombinationsTemp1.sol"} {:sourceLine 5} (true);
-assert {:first} {:sourceFile "/Users/etorres/Proyectos/verisol-test/2/new_folder1/CombinationsTemp1.sol"} {:sourceLine 7} (true);
+assert {:first} {:sourceFile "/Users/etorres/Proyectos/verisol-test/2/new_folder2/CombinationsTemp2.sol"} {:sourceLine 5} (true);
+assert {:first} {:sourceFile "/Users/etorres/Proyectos/verisol-test/2/new_folder2/CombinationsTemp2.sol"} {:sourceLine 7} (true);
 assume (((!(((StateEnum_SimpleMarketplace[this]) == (0)))) && ((StateEnum_SimpleMarketplace[this]) == (1))) && ((StateEnum_SimpleMarketplace[this]) == (1)));
-assert {:first} {:sourceFile "/Users/etorres/Proyectos/verisol-test/2/new_folder1/CombinationsTemp1.sol"} {:sourceLine 8} (true);
+assert {:first} {:sourceFile "/Users/etorres/Proyectos/verisol-test/2/new_folder2/CombinationsTemp2.sol"} {:sourceLine 8} (true);
 assume ((msgsender_MSG) == (InstanceOwner_SimpleMarketplace[this]));
-assert {:first} {:sourceFile "/Users/etorres/Proyectos/verisol-test/2/new_folder1/CombinationsTemp1.sol"} {:sourceLine 9} (true);
+assert {:first} {:sourceFile "/Users/etorres/Proyectos/verisol-test/2/new_folder2/CombinationsTemp2.sol"} {:sourceLine 9} (true);
 call Reject_SimpleMarketplace(this, msgsender_MSG, msgvalue_MSG);
-assert {:first} {:sourceFile "/Users/etorres/Proyectos/verisol-test/2/new_folder1/CombinationsTemp1.sol"} {:sourceLine 10} (true);
+assert {:first} {:sourceFile "/Users/etorres/Proyectos/verisol-test/2/new_folder2/CombinationsTemp2.sol"} {:sourceLine 10} (true);
 assert (!((((!(((StateEnum_SimpleMarketplace[this]) == (0)))) && ((StateEnum_SimpleMarketplace[this]) == (1))) && ((StateEnum_SimpleMarketplace[this]) == (1)))));
 }
 
@@ -91,7 +91,7 @@ var __var_1: Ref;
 assume ((msgsender_MSG) != (null));
 Balance[this] := 0;
 InstanceOwner_SimpleMarketplace[this] := null;
-Description_SimpleMarketplace[this] := -880227496;
+Description_SimpleMarketplace[this] := 581936576;
 AskingPrice_SimpleMarketplace[this] := 0;
 // Make array/mapping vars distinct for result
 call __var_1 := FreshRefGenerator();
@@ -108,17 +108,17 @@ call  {:cexpr "description"} boogie_si_record_sol2Bpl_int(description_s105);
 call  {:cexpr "price"} boogie_si_record_sol2Bpl_int(price_s105);
 call  {:cexpr "sender"} boogie_si_record_sol2Bpl_ref(sender_s105);
 call  {:cexpr "_verisolLastArg"} boogie_si_record_sol2Bpl_bool(true);
-assert {:first} {:sourceFile "/Users/etorres/Proyectos/verisol-test/2/new_folder1/CombinationsTemp1.sol"} {:sourceLine 29} (true);
-assert {:first} {:sourceFile "/Users/etorres/Proyectos/verisol-test/2/new_folder1/CombinationsTemp1.sol"} {:sourceLine 30} (true);
+assert {:first} {:sourceFile "/Users/etorres/Proyectos/verisol-test/2/new_folder2/CombinationsTemp2.sol"} {:sourceLine 29} (true);
+assert {:first} {:sourceFile "/Users/etorres/Proyectos/verisol-test/2/new_folder2/CombinationsTemp2.sol"} {:sourceLine 30} (true);
 InstanceOwner_SimpleMarketplace[this] := sender_s105;
 call  {:cexpr "InstanceOwner"} boogie_si_record_sol2Bpl_ref(InstanceOwner_SimpleMarketplace[this]);
-assert {:first} {:sourceFile "/Users/etorres/Proyectos/verisol-test/2/new_folder1/CombinationsTemp1.sol"} {:sourceLine 31} (true);
+assert {:first} {:sourceFile "/Users/etorres/Proyectos/verisol-test/2/new_folder2/CombinationsTemp2.sol"} {:sourceLine 31} (true);
 AskingPrice_SimpleMarketplace[this] := price_s105;
 call  {:cexpr "AskingPrice"} boogie_si_record_sol2Bpl_int(AskingPrice_SimpleMarketplace[this]);
-assert {:first} {:sourceFile "/Users/etorres/Proyectos/verisol-test/2/new_folder1/CombinationsTemp1.sol"} {:sourceLine 32} (true);
+assert {:first} {:sourceFile "/Users/etorres/Proyectos/verisol-test/2/new_folder2/CombinationsTemp2.sol"} {:sourceLine 32} (true);
 Description_SimpleMarketplace[this] := description_s105;
 call  {:cexpr "Description"} boogie_si_record_sol2Bpl_int(Description_SimpleMarketplace[this]);
-assert {:first} {:sourceFile "/Users/etorres/Proyectos/verisol-test/2/new_folder1/CombinationsTemp1.sol"} {:sourceLine 33} (true);
+assert {:first} {:sourceFile "/Users/etorres/Proyectos/verisol-test/2/new_folder2/CombinationsTemp2.sol"} {:sourceLine 33} (true);
 StateEnum_SimpleMarketplace[this] := 0;
 }
 
@@ -146,32 +146,32 @@ call  {:cexpr "msg.sender"} boogie_si_record_sol2Bpl_ref(msgsender_MSG);
 call  {:cexpr "msg.value"} boogie_si_record_sol2Bpl_int(msgvalue_MSG);
 call  {:cexpr "offerPrice"} boogie_si_record_sol2Bpl_int(offerPrice_s151);
 call  {:cexpr "_verisolLastArg"} boogie_si_record_sol2Bpl_bool(true);
-assert {:first} {:sourceFile "/Users/etorres/Proyectos/verisol-test/2/new_folder1/CombinationsTemp1.sol"} {:sourceLine 37} (true);
-assert {:first} {:sourceFile "/Users/etorres/Proyectos/verisol-test/2/new_folder1/CombinationsTemp1.sol"} {:sourceLine 38} (true);
+assert {:first} {:sourceFile "/Users/etorres/Proyectos/verisol-test/2/new_folder2/CombinationsTemp2.sol"} {:sourceLine 37} (true);
+assert {:first} {:sourceFile "/Users/etorres/Proyectos/verisol-test/2/new_folder2/CombinationsTemp2.sol"} {:sourceLine 38} (true);
 if ((offerPrice_s151) == (0)) {
-assert {:first} {:sourceFile "/Users/etorres/Proyectos/verisol-test/2/new_folder1/CombinationsTemp1.sol"} {:sourceLine 39} (true);
-assert {:first} {:sourceFile "/Users/etorres/Proyectos/verisol-test/2/new_folder1/CombinationsTemp1.sol"} {:sourceLine 40} (true);
+assert {:first} {:sourceFile "/Users/etorres/Proyectos/verisol-test/2/new_folder2/CombinationsTemp2.sol"} {:sourceLine 39} (true);
+assert {:first} {:sourceFile "/Users/etorres/Proyectos/verisol-test/2/new_folder2/CombinationsTemp2.sol"} {:sourceLine 40} (true);
 assume (false);
 }
-assert {:first} {:sourceFile "/Users/etorres/Proyectos/verisol-test/2/new_folder1/CombinationsTemp1.sol"} {:sourceLine 43} (true);
+assert {:first} {:sourceFile "/Users/etorres/Proyectos/verisol-test/2/new_folder2/CombinationsTemp2.sol"} {:sourceLine 43} (true);
 if ((StateEnum_SimpleMarketplace[this]) != (0)) {
-assert {:first} {:sourceFile "/Users/etorres/Proyectos/verisol-test/2/new_folder1/CombinationsTemp1.sol"} {:sourceLine 44} (true);
-assert {:first} {:sourceFile "/Users/etorres/Proyectos/verisol-test/2/new_folder1/CombinationsTemp1.sol"} {:sourceLine 45} (true);
+assert {:first} {:sourceFile "/Users/etorres/Proyectos/verisol-test/2/new_folder2/CombinationsTemp2.sol"} {:sourceLine 44} (true);
+assert {:first} {:sourceFile "/Users/etorres/Proyectos/verisol-test/2/new_folder2/CombinationsTemp2.sol"} {:sourceLine 45} (true);
 assume (false);
 }
-assert {:first} {:sourceFile "/Users/etorres/Proyectos/verisol-test/2/new_folder1/CombinationsTemp1.sol"} {:sourceLine 48} (true);
+assert {:first} {:sourceFile "/Users/etorres/Proyectos/verisol-test/2/new_folder2/CombinationsTemp2.sol"} {:sourceLine 48} (true);
 if ((InstanceOwner_SimpleMarketplace[this]) == (msgsender_MSG)) {
-assert {:first} {:sourceFile "/Users/etorres/Proyectos/verisol-test/2/new_folder1/CombinationsTemp1.sol"} {:sourceLine 49} (true);
-assert {:first} {:sourceFile "/Users/etorres/Proyectos/verisol-test/2/new_folder1/CombinationsTemp1.sol"} {:sourceLine 50} (true);
+assert {:first} {:sourceFile "/Users/etorres/Proyectos/verisol-test/2/new_folder2/CombinationsTemp2.sol"} {:sourceLine 49} (true);
+assert {:first} {:sourceFile "/Users/etorres/Proyectos/verisol-test/2/new_folder2/CombinationsTemp2.sol"} {:sourceLine 50} (true);
 assume (false);
 }
-assert {:first} {:sourceFile "/Users/etorres/Proyectos/verisol-test/2/new_folder1/CombinationsTemp1.sol"} {:sourceLine 53} (true);
+assert {:first} {:sourceFile "/Users/etorres/Proyectos/verisol-test/2/new_folder2/CombinationsTemp2.sol"} {:sourceLine 53} (true);
 InstanceBuyer_SimpleMarketplace[this] := msgsender_MSG;
 call  {:cexpr "InstanceBuyer"} boogie_si_record_sol2Bpl_ref(InstanceBuyer_SimpleMarketplace[this]);
-assert {:first} {:sourceFile "/Users/etorres/Proyectos/verisol-test/2/new_folder1/CombinationsTemp1.sol"} {:sourceLine 54} (true);
+assert {:first} {:sourceFile "/Users/etorres/Proyectos/verisol-test/2/new_folder2/CombinationsTemp2.sol"} {:sourceLine 54} (true);
 OfferPrice_SimpleMarketplace[this] := offerPrice_s151;
 call  {:cexpr "OfferPrice"} boogie_si_record_sol2Bpl_int(OfferPrice_SimpleMarketplace[this]);
-assert {:first} {:sourceFile "/Users/etorres/Proyectos/verisol-test/2/new_folder1/CombinationsTemp1.sol"} {:sourceLine 55} (true);
+assert {:first} {:sourceFile "/Users/etorres/Proyectos/verisol-test/2/new_folder2/CombinationsTemp2.sol"} {:sourceLine 55} (true);
 StateEnum_SimpleMarketplace[this] := 1;
 }
 
@@ -183,20 +183,20 @@ call  {:cexpr "this"} boogie_si_record_sol2Bpl_ref(this);
 call  {:cexpr "msg.sender"} boogie_si_record_sol2Bpl_ref(msgsender_MSG);
 call  {:cexpr "msg.value"} boogie_si_record_sol2Bpl_int(msgvalue_MSG);
 call  {:cexpr "_verisolLastArg"} boogie_si_record_sol2Bpl_bool(true);
-assert {:first} {:sourceFile "/Users/etorres/Proyectos/verisol-test/2/new_folder1/CombinationsTemp1.sol"} {:sourceLine 59} (true);
-assert {:first} {:sourceFile "/Users/etorres/Proyectos/verisol-test/2/new_folder1/CombinationsTemp1.sol"} {:sourceLine 60} (true);
+assert {:first} {:sourceFile "/Users/etorres/Proyectos/verisol-test/2/new_folder2/CombinationsTemp2.sol"} {:sourceLine 59} (true);
+assert {:first} {:sourceFile "/Users/etorres/Proyectos/verisol-test/2/new_folder2/CombinationsTemp2.sol"} {:sourceLine 60} (true);
 if ((StateEnum_SimpleMarketplace[this]) != (1)) {
-assert {:first} {:sourceFile "/Users/etorres/Proyectos/verisol-test/2/new_folder1/CombinationsTemp1.sol"} {:sourceLine 61} (true);
-assert {:first} {:sourceFile "/Users/etorres/Proyectos/verisol-test/2/new_folder1/CombinationsTemp1.sol"} {:sourceLine 62} (true);
+assert {:first} {:sourceFile "/Users/etorres/Proyectos/verisol-test/2/new_folder2/CombinationsTemp2.sol"} {:sourceLine 61} (true);
+assert {:first} {:sourceFile "/Users/etorres/Proyectos/verisol-test/2/new_folder2/CombinationsTemp2.sol"} {:sourceLine 62} (true);
 assume (false);
 }
-assert {:first} {:sourceFile "/Users/etorres/Proyectos/verisol-test/2/new_folder1/CombinationsTemp1.sol"} {:sourceLine 65} (true);
+assert {:first} {:sourceFile "/Users/etorres/Proyectos/verisol-test/2/new_folder2/CombinationsTemp2.sol"} {:sourceLine 65} (true);
 if ((InstanceOwner_SimpleMarketplace[this]) != (msgsender_MSG)) {
-assert {:first} {:sourceFile "/Users/etorres/Proyectos/verisol-test/2/new_folder1/CombinationsTemp1.sol"} {:sourceLine 66} (true);
-assert {:first} {:sourceFile "/Users/etorres/Proyectos/verisol-test/2/new_folder1/CombinationsTemp1.sol"} {:sourceLine 67} (true);
+assert {:first} {:sourceFile "/Users/etorres/Proyectos/verisol-test/2/new_folder2/CombinationsTemp2.sol"} {:sourceLine 66} (true);
+assert {:first} {:sourceFile "/Users/etorres/Proyectos/verisol-test/2/new_folder2/CombinationsTemp2.sol"} {:sourceLine 67} (true);
 assume (false);
 }
-assert {:first} {:sourceFile "/Users/etorres/Proyectos/verisol-test/2/new_folder1/CombinationsTemp1.sol"} {:sourceLine 71} (true);
+assert {:first} {:sourceFile "/Users/etorres/Proyectos/verisol-test/2/new_folder2/CombinationsTemp2.sol"} {:sourceLine 71} (true);
 StateEnum_SimpleMarketplace[this] := 0;
 }
 
@@ -208,20 +208,20 @@ call  {:cexpr "this"} boogie_si_record_sol2Bpl_ref(this);
 call  {:cexpr "msg.sender"} boogie_si_record_sol2Bpl_ref(msgsender_MSG);
 call  {:cexpr "msg.value"} boogie_si_record_sol2Bpl_int(msgvalue_MSG);
 call  {:cexpr "_verisolLastArg"} boogie_si_record_sol2Bpl_bool(true);
-assert {:first} {:sourceFile "/Users/etorres/Proyectos/verisol-test/2/new_folder1/CombinationsTemp1.sol"} {:sourceLine 75} (true);
-assert {:first} {:sourceFile "/Users/etorres/Proyectos/verisol-test/2/new_folder1/CombinationsTemp1.sol"} {:sourceLine 76} (true);
+assert {:first} {:sourceFile "/Users/etorres/Proyectos/verisol-test/2/new_folder2/CombinationsTemp2.sol"} {:sourceLine 75} (true);
+assert {:first} {:sourceFile "/Users/etorres/Proyectos/verisol-test/2/new_folder2/CombinationsTemp2.sol"} {:sourceLine 76} (true);
 if ((StateEnum_SimpleMarketplace[this]) != (1)) {
-assert {:first} {:sourceFile "/Users/etorres/Proyectos/verisol-test/2/new_folder1/CombinationsTemp1.sol"} {:sourceLine 77} (true);
-assert {:first} {:sourceFile "/Users/etorres/Proyectos/verisol-test/2/new_folder1/CombinationsTemp1.sol"} {:sourceLine 78} (true);
+assert {:first} {:sourceFile "/Users/etorres/Proyectos/verisol-test/2/new_folder2/CombinationsTemp2.sol"} {:sourceLine 77} (true);
+assert {:first} {:sourceFile "/Users/etorres/Proyectos/verisol-test/2/new_folder2/CombinationsTemp2.sol"} {:sourceLine 78} (true);
 assume (false);
 }
-assert {:first} {:sourceFile "/Users/etorres/Proyectos/verisol-test/2/new_folder1/CombinationsTemp1.sol"} {:sourceLine 81} (true);
+assert {:first} {:sourceFile "/Users/etorres/Proyectos/verisol-test/2/new_folder2/CombinationsTemp2.sol"} {:sourceLine 81} (true);
 if ((msgsender_MSG) != (InstanceOwner_SimpleMarketplace[this])) {
-assert {:first} {:sourceFile "/Users/etorres/Proyectos/verisol-test/2/new_folder1/CombinationsTemp1.sol"} {:sourceLine 82} (true);
-assert {:first} {:sourceFile "/Users/etorres/Proyectos/verisol-test/2/new_folder1/CombinationsTemp1.sol"} {:sourceLine 83} (true);
+assert {:first} {:sourceFile "/Users/etorres/Proyectos/verisol-test/2/new_folder2/CombinationsTemp2.sol"} {:sourceLine 82} (true);
+assert {:first} {:sourceFile "/Users/etorres/Proyectos/verisol-test/2/new_folder2/CombinationsTemp2.sol"} {:sourceLine 83} (true);
 assume (false);
 }
-assert {:first} {:sourceFile "/Users/etorres/Proyectos/verisol-test/2/new_folder1/CombinationsTemp1.sol"} {:sourceLine 86} (true);
+assert {:first} {:sourceFile "/Users/etorres/Proyectos/verisol-test/2/new_folder2/CombinationsTemp2.sol"} {:sourceLine 86} (true);
 StateEnum_SimpleMarketplace[this] := 2;
 }
 
